CertiGC/gc_spec.v
@@ -35,13 +35,6 @@ Definition all_string_constants (sh: share) (gv: globals) : mpred :=
   cstring sh (map init_data2byte (gvar_init v___stringlit_14)) (gv ___stringlit_14) *
   cstring sh (map init_data2byte (gvar_init v___stringlit_15)) (gv ___stringlit_15).
 
-  (*  obsolete?
-Definition MSS_constant (gv: globals): mpred :=
-  data_at Ews (if Archi.ptr64 then tulong else tuint)
-          (if Archi.ptr64 then Vlong (Int64.repr MAX_SPACE_SIZE) else
-             Vint (Int.repr MAX_SPACE_SIZE)) (gv _MAX_SPACE_SIZE).
-*)
-
 Definition test_int_or_ptr_spec :=
  DECLARE _test_int_or_ptr
  WITH x : val
@@ -343,12 +336,11 @@ Definition create_space_spec :=
           0 <= n <= MAX_SPACE_SIZE)
     PARAMS (s; if Archi.ptr64 then Vlong (Int64.repr n) else Vint (Int.repr n))
     GLOBALS (gv)
-    SEP (mem_mgr gv; all_string_constants rsh gv; data_at_ sh space_type s (*;
-        MSS_constant gv*))
+    SEP (mem_mgr gv; all_string_constants rsh gv; data_at_ sh space_type s)
   POST [tvoid]
     EX p: val,
     PROP () LOCAL ()
-    SEP (mem_mgr gv; all_string_constants rsh gv; (*MSS_constant gv;*)
+    SEP (mem_mgr gv; all_string_constants rsh gv;
          malloc_token Ews (tarray int_or_ptr_type n) p;
          data_at_ Ews (tarray int_or_ptr_type n) p;
          data_at sh space_type (p, (p, (offset_val (WORD_SIZE * n) p,offset_val (WORD_SIZE * n) p))) s).
@@ -362,11 +354,11 @@ Definition create_heap_spec :=
     PROP (readable_share sh)
     PARAMS ()
     GLOBALS (gv)
-    SEP (mem_mgr gv; all_string_constants sh gv(*; MSS_constant gv*))
+    SEP (mem_mgr gv; all_string_constants sh gv)
   POST [tptr heap_type]
     EX h: val, EX p: val,
     PROP () LOCAL (temp ret_temp h)
-    SEP (mem_mgr gv; all_string_constants sh gv; (*MSS_constant gv;*)
+    SEP (mem_mgr gv; all_string_constants sh gv;
         malloc_token Ews heap_type h;
          data_at Ews heap_type
                  ((p, (p, (offset_val (WORD_SIZE * NURSERY_SIZE) p,offset_val (WORD_SIZE * NURSERY_SIZE) p)))
@@ -381,11 +373,11 @@ Definition make_tinfo_spec :=
     PROP (readable_share sh)
     PARAMS ()
     GLOBALS (gv)
-    SEP (mem_mgr gv; all_string_constants sh gv(*; MSS_constant gv*))
+    SEP (mem_mgr gv; all_string_constants sh gv)
   POST [tptr thread_info_type]
     EX t: val, EX h: val, EX p: val,
     PROP () LOCAL (temp ret_temp t)
-    SEP (mem_mgr gv; all_string_constants sh gv; (*MSS_constant gv;*)
+    SEP (mem_mgr gv; all_string_constants sh gv;
          malloc_token Ews thread_info_type t;
          data_at Ews thread_info_type
                  (p, (offset_val (WORD_SIZE * NURSERY_SIZE) p,
@@ -428,12 +420,12 @@ Definition garbage_collect_spec :=
   PRE [tptr thread_info_type]
     PROP (readable_share rsh; writable_share sh;
           super_compatible g (ti_heap t_info) (frames2rootpairs (ti_frames t_info)) roots outlier;
-          garbage_collect_condition g (ti_heap t_info) roots;
+          garbage_collect_condition g (ti_heap t_info);
           safe_to_copy g)
     PARAMS (ti)
     GLOBALS (gv)
     SEP (mem_mgr gv;
-         all_string_constants rsh gv; (*MSS_constant gv;*)
+         all_string_constants rsh gv;
          outlier_rep outlier;
          graph_rep g;
          before_gc_thread_info_rep sh t_info ti;
@@ -442,14 +434,14 @@ Definition garbage_collect_spec :=
     EX g': LGraph, EX t_info': thread_info, EX roots': roots_t,
     PROP (super_compatible g' (ti_heap t_info') (frames2rootpairs (ti_frames t_info')) roots' outlier;
           garbage_collect_relation roots roots' g g';
-          garbage_collect_condition g' (ti_heap t_info') roots';
+          garbage_collect_condition g' (ti_heap t_info');
           safe_to_copy g';
           frame_shells_eq (ti_frames t_info) (ti_frames t_info');
           Ptrofs.unsigned (ti_nalloc t_info) <= 
                  total_space (heap_head (ti_heap t_info'))
                     - used_space (heap_head (ti_heap t_info')))
     LOCAL ()
-    SEP (mem_mgr gv; (*MSS_constant gv;*)
+    SEP (mem_mgr gv;
          all_string_constants rsh gv;
          outlier_rep outlier;
          graph_rep g';
